DH example trace and crypto predicates; DH security lemmas

examples/dh/DY.Example.DH.Protocol.Stateful.fst
@@ -9,10 +9,10 @@ open DY.Example.DH.Protocol.Total
 
 [@@ with_bytes bytes]
 type dh_session =
-    | InitiatorSentMsg1: b:principal -> x:bytes -> dh_session
-    | ResponderSentMsg2: a:principal -> gx:bytes -> gy:bytes -> y:bytes -> dh_session
-    | InitiatorSendMsg3: b:principal -> gx:bytes -> gy:bytes -> x:bytes -> dh_session
-    | ResponderReceivedMsg3: a:principal -> gx:bytes -> gy:bytes -> y:bytes -> dh_session
+  | InitiatorSentMsg1: b:principal -> x:bytes -> dh_session
+  | ResponderSentMsg2: a:principal -> gx:bytes -> gy:bytes -> y:bytes -> dh_session
+  | InitiatorSendMsg3: b:principal -> gx:bytes -> gy:bytes -> k:bytes -> dh_session
+  | ResponderReceivedMsg3: a:principal -> gx:bytes -> gy:bytes -> k:bytes -> dh_session
 
 %splice [ps_dh_session] (gen_parser (`dh_session))
 %splice [ps_dh_session_is_well_formed] (gen_is_well_formed_lemma (`dh_session))
@@ -25,8 +25,8 @@ instance dh_session_parseable_serializeable: parseable_serializeable bytes dh_se
 type dh_event =
   | Initiate1: a:principal -> b:principal -> x:bytes -> dh_event
   | Respond1: a:principal -> b:principal -> gx:bytes -> gy:bytes -> y:bytes -> dh_event
-  | Initiate2: a:principal -> b:principal -> gx:bytes -> gy:bytes -> x:bytes -> dh_event
-  | Respond2: a:principal -> b:principal -> gx:bytes -> gy:bytes -> y:bytes -> dh_event
+  | Initiate2: a:principal -> b:principal -> gx:bytes -> gy:bytes -> k:bytes -> dh_event
+  | Respond2: a:principal -> b:principal -> gx:bytes -> gy:bytes -> k:bytes -> dh_event
 
 %splice [ps_dh_event] (gen_parser (`dh_event))
 %splice [ps_dh_event_is_well_formed] (gen_is_well_formed_lemma (`dh_event))
@@ -42,8 +42,8 @@ val dh_session_label: string
 let dh_session_label = "DH.Session"
 
 type dh_global_sess_ids = {
-    pki: nat;
-    private_keys: nat;
+  pki: nat;
+  private_keys: nat;
 }
 
 (*** Stateful code ***)
@@ -56,94 +56,96 @@ type dh_global_sess_ids = {
 // a message over the network.
 val prepare_msg1: principal -> principal -> crypto nat
 let prepare_msg1 alice bob =
-    let* x = mk_rand NoUsage (join (principal_label alice) (principal_label bob)) 32 in
-    trigger_event alice (Initiate1 alice bob x);*
-    let* session_id = new_session_id alice in
-    set_typed_state dh_session_label alice session_id (InitiatorSentMsg1 bob x <: dh_session);*
-    return session_id
+  let* session_id = new_session_id alice in
+  let* x = mk_rand (DhKey "DH.dh_key") (principal_state_label alice session_id) 32 in
+  trigger_event alice (Initiate1 alice bob x);*
+  set_typed_state dh_session_label alice session_id (InitiatorSentMsg1 bob x <: dh_session);*
+  return session_id
 
 // Alice sends message 1
 val send_msg1: principal -> nat -> crypto (option nat)
 let send_msg1 alice session_id =
-    let*? session_state: dh_session = get_typed_state dh_session_label alice session_id in
-    match session_state with
-    | InitiatorSentMsg1 bob x -> (
-        let msg = compute_message1 bob x in
-        let* msg_id = send_msg msg in
-        return (Some msg_id)
-    )
-    | _ -> return None
+  let*? session_state: dh_session = get_typed_state dh_session_label alice session_id in
+  match session_state with
+  | InitiatorSentMsg1 bob x -> (
+    let msg = compute_message1 bob x in
+    let* msg_id = send_msg msg in
+    return (Some msg_id)
+  )
+  | _ -> return None
 
 // Bob prepares message 2
 val prepare_msg2: principal -> principal -> nat -> crypto (option nat)
 let prepare_msg2 alice bob msg_id =
-    let*? msg = recv_msg msg_id in
-    let*? msg1: message1 = return (decode_message1 msg) in
-    let* y = mk_rand NoUsage (join (principal_label alice) (principal_label bob)) 32 in
-    let gy = dh_pk y in
-    trigger_event bob (Respond1 alice bob msg1.gx gy y);*
-    let* session_id = new_session_id bob in
-    set_typed_state dh_session_label bob session_id (ResponderSentMsg2 alice msg1.gx gy y <: dh_session);*
-    return (Some session_id)
+  let*? msg = recv_msg msg_id in
+  let*? msg1: message1 = return (decode_message1 msg) in
+  let* session_id = new_session_id bob in
+  let* y = mk_rand (DhKey "DH.dh_key") (principal_state_label bob session_id) 32 in
+  let gy = dh_pk y in
+  trigger_event bob (Respond1 alice bob msg1.gx gy y);*
+  set_typed_state dh_session_label bob session_id (ResponderSentMsg2 alice msg1.gx gy y <: dh_session);*
+  return (Some session_id)
 
 // Bob sends message 2
 val send_msg2: dh_global_sess_ids -> principal -> nat -> crypto (option nat)
 let send_msg2 global_sess_id bob session_id =
-    let*? session_state: dh_session = get_typed_state dh_session_label bob session_id in
-    match session_state with
-    | ResponderSentMsg2 alice gx gy y -> (
-        let*? sk_b = get_private_key bob global_sess_id.private_keys (Sign "DH.SigningKey") in
-        let* n_sig = mk_rand SigNonce (principal_label bob) 32 in
-        let msg = compute_message2 alice bob gx gy sk_b n_sig in
-        let* msg_id = send_msg msg in
-        return (Some msg_id)
-    )
-    | _ -> return None
+  let*? session_state: dh_session = get_typed_state dh_session_label bob session_id in
+  match session_state with
+  | ResponderSentMsg2 alice gx gy y -> (
+    let*? sk_b = get_private_key bob global_sess_id.private_keys (Sign "DH.SigningKey") in
+    let* n_sig = mk_rand SigNonce (principal_label bob) 32 in
+    let msg = compute_message2 alice bob gx gy sk_b n_sig in
+    let* msg_id = send_msg msg in
+    return (Some msg_id)
+  )
+  | _ -> return None
 
 // Alice prepares message 3
 //
 // This function has to verify the signature from message 2
 val prepare_msg3: dh_global_sess_ids -> principal -> principal -> nat -> nat -> crypto (option unit)
 let prepare_msg3 global_sess_id alice bob msg_id session_id =
-    let*? session_state: dh_session = get_typed_state dh_session_label alice session_id in
-    match session_state with
-    | InitiatorSentMsg1 bob x -> (
-        let*? pk_b = get_public_key alice global_sess_id.pki (Verify "DH.SigningKey") bob in
-        let*? msg = recv_msg msg_id in
-        let gx = dh_pk x in
-        let*? msg2: message2 = return (decode_message2 msg alice gx pk_b) in
-        trigger_event alice (Initiate2 alice bob gx msg2.gy x);*
-        set_typed_state dh_session_label alice session_id (InitiatorSendMsg3 bob gx msg2.gy x <: dh_session);*
-        return (Some ())
-    )
-    | _ -> return None
+  let*? session_state: dh_session = get_typed_state dh_session_label alice session_id in
+  match session_state with
+  | InitiatorSentMsg1 bob x -> (
+    let*? pk_b = get_public_key alice global_sess_id.pki (Verify "DH.SigningKey") bob in
+    let*? msg = recv_msg msg_id in
+    let gx = dh_pk x in
+    let*? msg2: message2 = return (decode_message2 msg alice gx pk_b) in
+    let k = dh x msg2.gy in
+    trigger_event alice (Initiate2 alice bob gx msg2.gy k);*
+    set_typed_state dh_session_label alice session_id (InitiatorSendMsg3 bob gx msg2.gy k <: dh_session);*
+    return (Some ())
+  )
+  | _ -> return None
 
 // Alice send message 3
 val send_msg3: dh_global_sess_ids -> principal -> principal -> nat -> crypto (option nat)
 let send_msg3 global_sess_id alice bob session_id =
-    let*? session_state: dh_session = get_typed_state dh_session_label alice session_id in
-    match session_state with
-    | InitiatorSendMsg3 bob gx gy x -> (
-        let*? sk_a = get_private_key alice global_sess_id.private_keys (Sign "DH.SigningKey") in
-        let* n_sig = mk_rand SigNonce (principal_label alice) 32 in
-        let msg = compute_message3 alice bob gx gy sk_a n_sig in
-        let* msg_id = send_msg msg in
-        return (Some msg_id)
-    )
-    | _ -> return None
+  let*? session_state: dh_session = get_typed_state dh_session_label alice session_id in
+  match session_state with
+  | InitiatorSendMsg3 bob gx gy x -> (
+    let*? sk_a = get_private_key alice global_sess_id.private_keys (Sign "DH.SigningKey") in
+    let* n_sig = mk_rand SigNonce (principal_label alice) 32 in
+    let msg = compute_message3 alice bob gx gy sk_a n_sig in
+    let* msg_id = send_msg msg in
+    return (Some msg_id)
+  )
+  | _ -> return None
 
 // Bob verifies message 3
 val verify_msg3: dh_global_sess_ids -> principal -> principal -> nat -> nat -> crypto (option unit)
 let verify_msg3 global_sess_id alice bob msg_id session_id =
-    let*? session_state: dh_session = get_typed_state dh_session_label bob session_id in
-    match session_state with
-    | ResponderSentMsg2 alice gx gy y -> (
-        let*? pk_a = get_public_key bob global_sess_id.pki (Verify "DH.SigningKey") alice in
-        let*? msg = recv_msg msg_id in
-        let*? msg3: message3 = return (decode_message3 msg bob gx gy pk_a) in
-        trigger_event bob (Respond2 alice bob gx gy y);*
-        set_typed_state dh_session_label bob session_id (ResponderReceivedMsg3 alice gx gy y <: dh_session);*
-        return (Some ())
-    )
-    | _ -> return None
+  let*? session_state: dh_session = get_typed_state dh_session_label bob session_id in
+  match session_state with
+  | ResponderSentMsg2 alice gx gy y -> (
+    let*? pk_a = get_public_key bob global_sess_id.pki (Verify "DH.SigningKey") alice in
+    let*? msg = recv_msg msg_id in
+    let*? msg3: message3 = return (decode_message3 msg bob gx gy pk_a) in
+    let k = dh y gx in
+    trigger_event bob (Respond2 alice bob gx gy k);*
+    set_typed_state dh_session_label bob session_id (ResponderReceivedMsg3 alice gx gy k <: dh_session);*
+    return (Some ())
+  )
+  | _ -> return None
     
