examples/dh/DY.Example.DH.Protocol.Stateful.Proof.fst
@@ -1,0 +1,141 @@
+module DY.Example.DH.Protocol.Stateful.Proof
+
+open Comparse
+open DY.Core
+open DY.Lib
+open DY.Example.DH.Protocol.Total
+open DY.Example.DH.Protocol.Total.Proof
+open DY.Example.DH.Protocol.Stateful
+
+#set-options "--fuel 0 --ifuel 1 --z3rlimit 25  --z3cliopt 'smt.qi.eager_threshold=100'"
+
+(*** Trace invariants ***)
+
+/// The (local) state predicate.
+
+val is_dh_shared_key: trace -> principal -> principal -> bytes -> prop
+let is_dh_shared_key tr a b k = exists si sj.
+  is_secret (join (principal_state_label a si) (principal_state_label b sj)) tr k /\ 
+  get_usage k == AeadKey "DH.aead_key"
+
+let dh_session_pred: typed_session_pred dh_session = {
+  pred = (fun tr prin sess_id st ->
+    match st with
+    | InitiatorSentMsg1 bob x -> (
+      let alice = prin in
+      is_secret (principal_state_label alice sess_id) tr x /\
+      get_usage x == DhKey "DH.dh_key" /\
+      event_triggered tr alice (Initiate1 alice bob x)
+    )
+    | ResponderSentMsg2 alice gx gy y -> (
+      let bob = prin in
+      is_publishable tr gx /\ is_publishable tr gy /\
+      is_knowable_by (principal_state_label bob sess_id) tr y /\
+      is_secret (principal_state_label bob sess_id) tr y /\ get_usage y  == DhKey "DH.dh_key" /\
+      gy == dh_pk y /\
+      event_triggered tr bob (Respond1 alice bob gx gy y)
+    )
+    | InitiatorSendMsg3 bob gx gy k -> (
+      let alice = prin in
+      is_publishable tr gx /\ is_publishable tr gy /\
+      is_knowable_by (principal_state_label alice sess_id) tr k /\
+      event_triggered tr alice (Initiate2 alice bob gx gy k) /\
+      (is_corrupt tr (principal_state_label alice sess_id) \/
+      (exists y. k == dh y gx /\ is_dh_shared_key tr alice bob k /\ 
+        event_triggered tr bob (Respond1 alice bob gx gy y)))
+    )
+    | ResponderReceivedMsg3 alice gx gy k -> (
+      let bob = prin in
+      is_publishable tr gx /\ is_publishable tr gy /\
+      is_knowable_by (principal_state_label bob sess_id) tr k /\
+      event_triggered tr bob (Respond2 alice bob gx gy k) /\
+      (is_corrupt tr (principal_state_label bob sess_id) \/
+      is_dh_shared_key tr alice bob k /\ event_triggered tr alice (Initiate2 alice bob gx gy k))
+    )
+  );
+  pred_later = (fun tr1 tr2 prin sess_id st -> ());
+  pred_knowable = (fun tr prin sess_id st -> ());
+}
+
+/// The (local) event predicate.
+
+let dh_event_pred: event_predicate dh_event =
+  fun tr prin e ->
+    match e with
+    | Initiate1 alice bob x -> True
+    | Respond1 alice bob gx gy y -> (
+      is_publishable tr gx /\ is_publishable tr gy /\
+      (exists sess_id. is_secret (principal_state_label bob sess_id) tr y) /\
+      get_usage y == DhKey "DH.dh_key" /\
+      gy = dh_pk y
+    )
+    | Initiate2 alice bob gx gy k -> (
+      is_publishable tr gx /\ is_publishable tr gy /\
+      (exists x sess_id. is_secret (principal_state_label alice sess_id) tr x /\
+      gx = dh_pk x) /\
+      (is_corrupt tr (principal_label bob) \/
+      (exists y. k == dh y gx /\ is_dh_shared_key tr alice bob k /\ event_triggered tr bob (Respond1 alice bob gx gy y)))
+    )
+    | Respond2 alice bob gx gy k -> (
+      is_corrupt tr (principal_label alice) \/ 
+      (is_dh_shared_key tr alice bob k /\
+      event_triggered tr alice (Initiate2 alice bob gx gy k))
+    )
+
+(* Couldn't we hide all of the following code in a function returning a record? *)
+
+/// List of all local state predicates.
+
+let all_sessions = [
+  (pki_label, typed_session_pred_to_session_pred (map_session_invariant pki_pred));
+  (private_keys_label, typed_session_pred_to_session_pred (map_session_invariant private_keys_pred));
+  (dh_session_label, typed_session_pred_to_session_pred dh_session_pred);
+]
+
+/// List of all local event predicates.
+
+let all_events = [
+  (dh_event_instance.tag, compile_event_pred dh_event_pred)
+]
+
+/// Create the global trace invariants.
+
+let dh_trace_invs: trace_invariants (dh_crypto_invs) = {
+  state_pred = mk_state_predicate dh_crypto_invs all_sessions;
+  event_pred = mk_event_pred all_events;
+}
+
+instance dh_protocol_invs: protocol_invariants = {
+  crypto_invs = dh_crypto_invs;
+  trace_invs = dh_trace_invs;
+}
+
+/// Lemmas that the global state predicate contains all the local ones
+
+val all_sessions_has_all_sessions: unit -> Lemma (norm [delta_only [`%all_sessions; `%for_allP]; iota; zeta] (for_allP (has_session_pred dh_protocol_invs) all_sessions))
+let all_sessions_has_all_sessions () =
+  assert_norm(List.Tot.no_repeats_p (List.Tot.map fst (all_sessions)));
+  mk_global_session_pred_correct dh_protocol_invs all_sessions;
+  norm_spec [delta_only [`%all_sessions; `%for_allP]; iota; zeta] (for_allP (has_session_pred dh_protocol_invs) all_sessions)
+
+val full_dh_session_pred_has_pki_invariant: squash (has_pki_invariant dh_protocol_invs)
+let full_dh_session_pred_has_pki_invariant = all_sessions_has_all_sessions ()
+
+val full_dh_session_pred_has_private_keys_invariant: squash (has_private_keys_invariant dh_protocol_invs)
+let full_dh_session_pred_has_private_keys_invariant = all_sessions_has_all_sessions ()
+
+val full_dh_session_pred_has_nsl_invariant: squash (has_typed_session_pred dh_protocol_invs (dh_session_label, dh_session_pred))
+let full_dh_session_pred_has_nsl_invariant = all_sessions_has_all_sessions ()
+
+/// Lemmas that the global event predicate contains all the local ones
+
+val all_events_has_all_events: unit -> Lemma (norm [delta_only [`%all_events; `%for_allP]; iota; zeta] (for_allP (has_compiled_event_pred dh_protocol_invs) all_events))
+let all_events_has_all_events () =
+  assert_norm(List.Tot.no_repeats_p (List.Tot.map fst (all_events)));
+  mk_event_pred_correct dh_protocol_invs all_events;
+  norm_spec [delta_only [`%all_events; `%for_allP]; iota; zeta] (for_allP (has_compiled_event_pred dh_protocol_invs) all_events);
+  let dumb_lemma (x:prop) (y:prop): Lemma (requires x /\ x == y) (ensures y) = () in
+  dumb_lemma (for_allP (has_compiled_event_pred dh_protocol_invs) all_events) (norm [delta_only [`%all_events; `%for_allP]; iota; zeta] (for_allP (has_compiled_event_pred dh_protocol_invs) all_events))
+
+val full_nsl_event_pred_has_nsl_invariant: squash (has_event_pred dh_protocol_invs dh_event_pred)
+let full_nsl_event_pred_has_nsl_invariant = all_events_has_all_events ()
