examples/dh/DY.Example.DH.Protocol.Total.Proof.fst
@@ -1,0 +1,41 @@
+module DY.Example.DH.Protocol.Total.Proof
+
+open Comparse
+open DY.Core
+open DY.Lib
+open DY.Example.DH.Protocol.Total
+open DY.Example.DH.Protocol.Stateful
+
+(*** Cryptographic invariants ***)
+
+val dh_crypto_usages: crypto_usages
+instance dh_crypto_usages = default_crypto_usages
+
+#push-options "--ifuel 2 --fuel 0"
+val dh_crypto_preds: crypto_predicates dh_crypto_usages
+let dh_crypto_preds = {
+  default_crypto_predicates dh_crypto_usages with
+
+  sign_pred = (fun tr vk sig_msg -> 
+    get_signkey_usage vk == SigKey "DH.SigningKey" /\
+    (exists prin. get_signkey_label vk = principal_label prin /\ (
+      match parse sig_message sig_msg with
+      | Some (SigMsg2 sig_msg2) -> (
+        exists y. sig_msg2.gy == (dh_pk y) /\ event_triggered tr prin (Respond1 sig_msg2.a prin sig_msg2.gx sig_msg2.gy y)
+      )
+      | Some (SigMsg3 sig_msg3) -> (
+        exists x. sig_msg3.gx == (dh_pk x) /\ event_triggered tr prin (Initiate2 prin sig_msg3.b sig_msg3.gx sig_msg3.gy x)
+      )
+      | None -> False
+    ))
+  );
+  sign_pred_later = (fun tr1 tr2 vk msg -> ())
+}
+#pop-options
+
+instance dh_crypto_invs = {
+  usages = dh_crypto_usages;
+  preds = dh_crypto_preds;
+}
+
+(*** Proofs ***)
