examples/dh/DY.Example.DH.Protocol.Total.fst
@@ -17,8 +17,8 @@ open DY.Lib
 // Annotation is needed for comparse to generate serialization methods
 [@@ with_bytes bytes]
 type message1 = {
-    alice:principal;
-    gx:bytes;
+  alice:principal;
+  gx:bytes;
 }
 
 %splice [ps_message1] (gen_parser (`message1))
@@ -26,9 +26,9 @@ type message1 = {
 
 [@@ with_bytes bytes]
 type message2 = {
-    bob:principal;
-    gy:bytes;
-    sg:bytes;
+  bob:principal;
+  gy:bytes;
+  sg:bytes;
 }
 
 %splice [ps_message2] (gen_parser (`message2))
@@ -36,95 +36,117 @@ type message2 = {
 
 [@@ with_bytes bytes]
 type message3 = {
-    sg:bytes;
+  sg:bytes;
 }
 
 %splice [ps_message3] (gen_parser (`message3))
 %splice [ps_message3_is_well_formed] (gen_is_well_formed_lemma (`message3))
 
-[@@ with_bytes bytes]
-type signature_message = {
-    p:principal;
-    gx:bytes;
-    gy:bytes;
-}
-
-%splice [ps_signature_message] (gen_parser (`signature_message))
-%splice [ps_signature_message_is_well_formed] (gen_is_well_formed_lemma (`signature_message))
 
 [@@ with_bytes bytes]
 type message =
-    | Msg1: msg:message1 -> message
-    | Msg2: msg:message2 -> message
-    | Msg3: msg:message3 -> message
-    | Sig: sig:signature_message -> message
+  | Msg1: msg:message1 -> message
+  | Msg2: msg:message2 -> message
+  | Msg3: msg:message3 -> message
 
 %splice [ps_message] (gen_parser (`message))
 %splice [ps_message_is_well_formed] (gen_is_well_formed_lemma (`message))
 
 instance parseable_serializeable_message: parseable_serializeable bytes message = mk_parseable_serializeable ps_message
 
+// Definition of signature terms
+[@@ with_bytes bytes]
+type sig_message2 = {
+  a:principal;
+  gx:bytes;
+  gy:bytes;
+}
+
+%splice [ps_sig_message2] (gen_parser (`sig_message2))
+%splice [ps_sig_message2_is_well_formed] (gen_is_well_formed_lemma (`sig_message2))
+
+[@@ with_bytes bytes]
+type sig_message3 = {
+  b:principal;
+  gx:bytes;
+  gy:bytes;
+}
+
+%splice [ps_sig_message3] (gen_parser (`sig_message3))
+%splice [ps_sig_message3_is_well_formed] (gen_is_well_formed_lemma (`sig_message3))
+
+[@@ with_bytes bytes]
+type sig_message =
+  | SigMsg2: msg:sig_message2 -> sig_message
+  | SigMsg3: msg:sig_message3 -> sig_message
+
+%splice [ps_sig_message] (gen_parser (`sig_message))
+%splice [ps_sig_message_is_well_formed] (gen_is_well_formed_lemma (`sig_message))
+
+instance parseable_serializeable_sig_message: parseable_serializeable bytes sig_message = mk_parseable_serializeable ps_sig_message
+
+
 (*** Message Processing ***)
 
 // Alice generates message 1
 val compute_message1: principal -> bytes -> bytes
 let compute_message1 alice x =
-    let gx = dh_pk x in
-    let msg = Msg1 {alice; gx} in
-    serialize message msg
+  let gx = dh_pk x in
+  let msg = Msg1 {alice; gx} in
+  serialize message msg
 
 // Bob parses message 1
 val decode_message1: bytes -> option message1
 let decode_message1 msg1_bytes =
-    let? msg1 = parse message msg1_bytes in
-    // These lines are the...
-    guard (Msg1? msg1);?
-    Some (Msg1?.msg msg1)
-    // ...short version of the following match:
-    (*    
-    match msg1 with
-    | Msg1 msg -> Some msg
-    | _ -> None
-    *)
+  let? msg1 = parse message msg1_bytes in
+  // These lines are the...
+  guard (Msg1? msg1);?
+  Some (Msg1?.msg msg1)
+  // ...short version of the following match:
+  (*    
+  match msg1 with
+  | Msg1 msg -> Some msg
+  | _ -> None
+  *)
 
 // Bob generates message 2
 val compute_message2: principal -> principal -> bytes -> bytes -> bytes -> bytes -> bytes
 let compute_message2 alice bob gx gy sk_b n_sig =
-    let sig_msg = Sig {p=alice; gx; gy} in
-    let sg = sign sk_b n_sig (serialize message sig_msg) in
-    let msg = Msg2 {bob; gy; sg} in
-    serialize message msg
+  let sig_msg = SigMsg2 {a=alice; gx; gy} in
+  let sg = sign sk_b n_sig (serialize sig_message sig_msg) in
+  let msg = Msg2 {bob; gy; sg} in
+  serialize message msg
 
 // Alice parses message 2
 val decode_message2: bytes -> principal -> bytes -> bytes -> option message2
 let decode_message2 msg2_bytes alice gx pk_b =
-    let? msg2_parsed = parse message msg2_bytes in
-    guard (Msg2? msg2_parsed);?
-    let msg2 = Msg2?.msg msg2_parsed in
-    // Verify the signature contained in the message 2
-    // with the gy value from the message and the gx
-    // value from Alice's state.
-    let gy = msg2.gy in
-    let sig_msg = Sig {p=alice; gx; gy} in
-    if verify pk_b (serialize message sig_msg) msg2.sg then Some (msg2)
-    else None
+  let? msg2_parsed = parse message msg2_bytes in
+  guard (Msg2? msg2_parsed);?
+  let msg2 = Msg2?.msg msg2_parsed in
+  // Verify the signature contained in the message 2
+  // with the gy value from the message and the gx
+  // value from Alice's state.
+  let gy = msg2.gy in
+  let sig_msg = SigMsg2 {a=alice; gx; gy} in
+  if verify pk_b (serialize sig_message sig_msg) msg2.sg then Some (msg2)
+  else None
 
 // Alice generates message3
 val compute_message3: principal -> principal -> bytes -> bytes -> bytes -> bytes -> bytes
 let compute_message3 alice bob gx gy sk_a n_sig =
-    let sig_msg = Sig {p=bob; gx; gy} in
-    let sg = sign sk_a n_sig (serialize message sig_msg) in
-    let msg = Msg3 {sg} in
-    serialize message msg
+  let sig_msg = SigMsg3 {b=bob; gx; gy} in
+  let sg = sign sk_a n_sig (serialize sig_message sig_msg) in
+  let msg = Msg3 {sg} in
+  serialize message msg
 
 // Bob parses message3
 val decode_message3: bytes -> principal -> bytes -> bytes -> bytes -> option message3
 let decode_message3 msg3_bytes bob gx gy pk_a =
-    let? msg3_parsed = parse message msg3_bytes in
-    guard (Msg3? msg3_parsed);?
-    let msg3 = Msg3?.msg msg3_parsed in
-    // Verify the signature contained in message 3
-    // with the gx and gy values from Bob's state.
-    let sig_msg = Sig {p=bob; gx; gy} in
-    if verify pk_a (serialize message sig_msg) msg3.sg then Some (msg3)
-    else None
+  let? msg3_parsed = parse message msg3_bytes in
+  guard (Msg3? msg3_parsed);?
+  let msg3 = Msg3?.msg msg3_parsed in
+  // Verify the signature contained in message 3
+  // with the gx and gy values from Bob's state.
+  let sig_msg = SigMsg3 {b=bob; gx; gy} in
+  if verify pk_a (serialize sig_message sig_msg) msg3.sg then Some (msg3)
+  else None
