examples/dh/DY.Example.DH.SecurityProperties.fst
@@ -1,0 +1,78 @@
+module DY.Example.DH.SecurityProperties
+
+open Comparse
+open DY.Core
+open DY.Lib
+open DY.Example.DH.Protocol.Total.Proof
+open DY.Example.DH.Protocol.Stateful
+open DY.Example.DH.Protocol.Stateful.Proof
+
+#set-options "--fuel 8 --ifuel 8 --z3rlimit 25  --z3cliopt 'smt.qi.eager_threshold=100'"
+
+(*
+  TODO: In the intrinsic version we use method like corrupt_at
+  and did_event_occur_before. Do we need these method here too?
+*)
+val initiator_correspondence_lemma: tr:trace -> i:nat -> alice:principal -> bob:principal -> gx:bytes -> gy:bytes -> k:bytes ->
+  Lemma
+  (requires event_triggered_at tr i alice (Initiate2 alice bob gx gy k) /\ 
+    trace_invariant tr)
+  (ensures is_corrupt tr (principal_label bob) \/
+    (exists y. event_triggered tr bob (Respond1 alice bob gx gy y) /\
+    k == dh y gx)
+  )
+let initiator_correspondence_lemma tr i alice bob gx gy k = ()
+
+val responder_correspondence_lemma: tr:trace -> i:nat -> alice:principal -> bob:principal -> gx:bytes -> gy:bytes -> k:bytes ->
+  Lemma
+  (requires event_triggered_at tr i bob (Respond2 alice bob gx gy k) /\
+    trace_invariant tr)
+  (ensures is_corrupt tr (principal_label alice) \/ 
+    event_triggered tr alice (Initiate2 alice bob gx gy k))
+let responder_correspondence_lemma tr i alice bob gx gy k = ()
+
+val key_secrecy_lemma: tr:trace -> k:bytes -> alice:principal -> bob:principal ->
+  Lemma
+  (requires 
+    trace_invariant tr /\
+    attacker_knows tr k 
+  )
+  (ensures
+    forall si sj. is_secret (join (principal_state_label alice si) (principal_state_label bob sj)) tr k ==> 
+    (is_corrupt tr (principal_state_label alice si) \/ is_corrupt tr (principal_state_label bob sj))
+  )
+let key_secrecy_lemma tr k alice bob = attacker_only_knows_publishable_values tr k
+
+val initiator_forward_secrecy_lemma: 
+  tr:trace -> i:nat -> alice:principal -> bob:principal -> gx:bytes -> gy:bytes -> k:bytes ->
+  Lemma
+  (requires
+    trace_invariant tr /\
+    event_triggered_at tr i alice (Initiate2 alice bob gx gy k) /\
+    attacker_knows tr k
+  )
+  (ensures
+    is_corrupt tr (principal_label bob) \/
+    (exists si sj. is_secret (join (principal_state_label alice si) (principal_state_label bob sj)) tr k /\
+      (is_corrupt tr (principal_state_label alice si) \/ is_corrupt tr (principal_state_label bob sj))
+    )
+  )
+let initiator_forward_secrecy_lemma tr i alice bob gx gy k = 
+  attacker_only_knows_publishable_values tr k
+
+val responder_forward_secrecy_lemma: 
+  tr:trace -> i:nat -> alice:principal -> bob:principal -> gx:bytes -> gy:bytes -> k:bytes ->
+  Lemma
+  (requires
+    trace_invariant tr /\
+    event_triggered_at tr i bob (Respond2 alice bob gx gy k) /\
+    attacker_knows tr k
+  )
+  (ensures
+    is_corrupt tr (principal_label alice) \/
+    (exists si sj. is_secret (join (principal_state_label alice si) (principal_state_label bob sj)) tr k /\
+      (is_corrupt tr (principal_state_label alice si) \/ is_corrupt tr (principal_state_label bob sj))
+    )
+  )
+let responder_forward_secrecy_lemma tr i alice bob gx gy k = 
+  attacker_only_knows_publishable_values tr k
